src/Core/RISCVMachine.v
@@ -27,7 +27,6 @@ Require Import coqutil.Map.Z_keyed_SortedListMap.
 Require Import coqutil.Z.HexNotation.
 Require coqutil.Map.SortedList.
 
-
 Require Import Lia.
 
 From RecordUpdate Require Import RecordSet.
